Folding in Alley's contribution. Generalizing Indifferentiability.

sha3/proof/Sponge.ec
@@ -1,8 +1,7 @@
-require import Option Pair Int ABitstring NewList.
-require (*..*) AWord Indifferentiability.
+require import Option Pair Int Real NewList NewFSet NewFMap.
+require (*..*) AWord LazyRO IRO Indifferentiability.
 (* TODO: Clean up the Bitstring and Word theories
       -- Make use of those new versions. *)
-
 (*...*) import Dprod.
 (* TODO: Datatype definitions and distributions should
      be properly separated and reorganized. *)
@@ -35,34 +34,84 @@ proof leq0_length by smt.
 
 type state = block * capacity.
 
+(** Ideal Functionality **)
+clone import IRO as Functionality with
+  type from <- block list.
+
+(** The following is just lining up type definitions and defines the
+    Indifferentiability experiment. Importantly, it defines neither
+    ideal primitive nor ideal functionality: only their type. **)
 clone import Indifferentiability as Main with
-  type from0 <- state,
-  type to0   <- state,
-  op   d0    <- fun (x:state) => dblock * dcapacity,
-  type from1 <- block list * int,
-  type to1   <- bitstring,
-  op   d1    <- fun (x:block list * int) => DBitstring.dbitstring x.`2.
+  type p_in  <- state,
+  type p_out <- state,
+  type f_in  <- block list * int,
+  type f_out <- bool list.
 
-module Sponge (H : H.RO): Construction(H) = {
-  proc init = H.init
+(** Ideal Primitive for the Random Transformation case **)
+clone import LazyRO as Primitive with
+  type from <- state,
+  type to   <- state,
+  op   d    <- dblock * dcapacity.
 
-  proc hash(p : block list, n : int): bitstring = {
-    var z = ABitstring.zeros n;
+(*** TODO: deal with these.
+       - bitstrings should have conversions to and from bool list
+       - the generic RO should be defined somewhere else
+       - lining up names and types should be easier than it is... ***)
+op to_bits: block -> bool list.
+
+module RO_to_P (O : Types.RO) = {
+  proc init = O.init
+  proc oracle = O.hash
+}.
+
+module IRO_to_F (O : IRO): Functionality = {
+  proc init = O.init
+
+  (* proc oracle = O.hash
+       does not work because of input types not lining up...
+     I though this had been taken care of. *)
+  proc oracle(x : block list * int): bool list = {
+    var bs;
+    bs = O.hash(x.`1,x.`2);
+    return bs;
+  }
+}.
+
+(** We can now define the sponge construction **)
+module Sponge (P : Primitive): Construction(P) = {
+  proc init = P.init
+
+  proc oracle(p : block list, n : int): bool list = {
+    var z;
     var s = (Block.zeros,Capacity.zeros);
     var i = 0;
 
     if (size p >= 1 /\ nth witness p (size p - 1) <> Block.zeros) {
-      z = ABitstring.zeros 0;
+      z = [];
       while (p <> []) {
-        s = H.hash(s.`1 ^ head witness p,s.`2);
+        s = P.oracle(s.`1 ^ head witness p,s.`2);
         p = behead p;
       }
       while (i < n/%r) {
-        z = z || (to_bits s.`1);
-        s = H.hash(s);
+        z = z ++ (Self.to_bits s.`1); (* Typing by constraint would be nice *)
+        s = P.oracle(s);
       }
     }
 
-    return sub z 0 n;
+    return take n z;
   }
 }.
+
+(** TODO: ftn is in fact a function of N
+      (number of queries to the primitive interface) **)
+op ftn: real.
+
+module P = RO_to_P(Primitive.H).
+module F = IRO_to_F(IRO).
+
+lemma TransformationLemma (D <: Distinguisher) &m:
+  exists (S <: Simulator),
+    `|Pr[Indif(Sponge(P),P,D).main() @ &m: res]
+      - Pr[Indif(F,S(F),D).main() @ &m: res]|
+  < ftn.
+proof. admit. qed.
